\chapter{Benchmarking Suites}
\label{appendix:benchmarks}

\section{Synthesised Programs for the Graded Linear Synthesis Calculi}
\label{sec:linear-benchmarks}
This section includes the synthesised programs for the benchmarking problems in
Section~\ref{sec:linear-base-evaluation}. 

\subsection{Hilbert}
\begin{enumerate}
\item $\otimes$-Intro:
\begin{granule}
and : forall { a b : Type } . a -> b -> (a, b)
and x y = (x, y)
\end{granule}
\item $\otimes$-Elim: \\ 
\begin{granule}
and1 : forall { a b : Type } .  (a, b [0]) -> a
and1 (y, [u]) = y
    
and2 : forall { a b : Type } . (a [0], b) -> b
and2 ([u], z) = z
\end{granule}
\item $\oplus$-Intro: 
\begin{granule}
data Either a b = Left a | Right b

or1 : forall a b . a -> Either a b
or1 x = Left x

or2 : forall a b . b -> Either a b
or2 x = Right x
\end{granule}
\item $\oplus$-Elim: 
\begin{granule}
data Either a b = Left a | Right b

or3 : forall { a b c : Type }
    . (a -> c) [0..1] 
    -> (b -> c) [0..1] 
    -> (Either a b) 
    -> c
or3 [u] [v] (Right x6) = v x6;
or3 [u] [v] (Left x5) = u x5
\end{granule}
\item SKI: 
\begin{granule}
s : forall { a b c : Type } 
  . (a -> (b -> c)) 
  -> (a -> b) 
  -> a [2] 
  -> c
s x y [u] = (x u) (y u)
    
k : forall { a b : Type } . a -> b [0..1] -> a
k x [z] = x
    
i : forall { a : Type } . a -> a
i x = x
\end{granule}
\end{enumerate}


\subsection{Comp}
\begin{enumerate}
\item 0/1: 
\begin{granule}
comp-01 : forall { a b c : Type }
        . (a [] -> b []) [] 
        -> (b [] -> c []) [] 
        -> (a [] -> c) []
comp-01 [z] [u] = 
    [\v -> 
        let [w] = v in 
        let [q] = z [w] in 
        let [x9] = u [q] in 
        let [x11] = z [w] in x9]
\end{granule}
\item CBN: 
\begin{granule}
comp-cbn : forall { a b c : Type }
         . (a [] -> b) [] 
         -> (b [] -> c) [] -> a [] -> c
comp-cbn [u] [w] [v] = w [u [v]]
\end{granule}
\item CBV: 
\begin{granule}
comp-cbv : forall { a b c : Type }  . 
         (a [] -> b []) [] 
         -> (b [] -> c []) [] 
         -> (a [] -> c []) []
comp-cbv [z] [u] = 
    [\v -> 
        (\ [w] -> 
            [(\ [q] -> q) (u [(\ [x9] -> x9) (z [w])])]) v]
\end{granule}
\item coK-$\mathcal{R}$:
\begin{granule}
compGen : forall {k : Coeffect, n m : k, a b c : Type} 
        . (a [m] -> b) [n] 
        -> (b [n] -> c) 
        -> a [n * m] 
        -> c
compGen [u] y [v] = y [u [v]]
\end{granule}
\item coK-$\mathbb{N}$:
\begin{granule}
compNat : forall {n m : Nat, a b c : Type} 
     . (a [m] -> b) [n] 
     -> (b [n] -> c) 
     -> a [n * m] 
     -> c
compNat [u] y [v] = y [u [v]]
\end{granule}
\item lin:
\begin{granule}
lin : forall { a b c : Type }
     . (a -> b) 
     -> (b -> c) 
     -> a 
     -> c
lin x y z = y (x z)
\end{granule}
\end{enumerate}



\subsection{Dist}
\begin{enumerate}
\item $\otimes$-!:
\begin{granule}
pull : forall { a b : Type } . (a [], b []) -> (a, b) []
pull ([u], [v]) = [(u, v)]
\end{granule}
\item $\otimes$-$\mathbb{N}$:
\begin{granule}
pull : forall {a b : Type, n : Nat} 
     . (a [n], b [n]) 
     -> (a, b) [n]
pull ([u], [v]) = [(u, v)]
\end{granule}
\item $\otimes$-$\mathcal{R}$:
\begin{granule}
pull : forall {a b : Type, k : Coeffect, c : k} 
     . (a [c], b [c]) 
     -> (a, b) [c]
pull ([u], [v]) = [(u, v)]
\end{granule}
\item $\oplus$-!:
\begin{granule}
data Either a b = Left a | Right b

pull : forall { a b : Type }
     . Either (a []) (b []) 
     -> (Either a b) []
pull (Right [v]) = [Right v];
pull (Left [z]) = [Left z]
\end{granule}
\item $\oplus$-$\mathbb{N}$:
\begin{granule}
data Either a b = Left a | Right b

pull : forall {a b : Type, n : Nat} 
     . Either (a [n]) (b [n]) 
     -> (Either a b) [n]
pull (Right [v]) = [Right v];
pull (Left [z]) = [Left z]
\end{granule}
\item $\oplus$-$\mathcal{R}$:
\begin{granule}
data Either a b = Left a | Right b

pull : forall { a b : Type, k : Coeffect, c : k } 
     . Either (a [c]) (b [c]) 
     -> (Either a b) [c]
pull (Right [v]) = [Right v];
pull (Left [z]) = [Left z]
\end{granule}
\item $\multimap$-!:
\begin{granule}
push : forall { a b : Type }
     . (a -> b) [] 
     -> a [] 
     -> b []
push [z] [u] = [z u]
\end{granule}
\item $\multimap$-$\mathbb{N}$:
\begin{granule}
push : forall {a b : Type, c : Nat}
     . (a -> b) [c] 
     -> a [c] 
     -> b [c]
push [z] [u] = [z u]
\end{granule}
\item $\multimap$-$\mathcal{R}$:
\begin{granule}
push : forall { a b : Type, k : Coeffect, c : k } 
     . (a -> b) [c] 
     -> a [c] 
     -> b [c]
push [z] [u] = [z u]
\end{granule}
\end{enumerate}

\subsection{Vec}
\begin{enumerate}
\item vec5:
\begin{granule}
vec5 : forall { a b : Type }
     . (a -> b) [5] 
     -> ((((a, a), a), a), a) 
     -> ((((b, b), b), b), b)
vec5 [z] ((((x9, x10), x8), x6), x4) = 
    ((((z x9, z x8), z x6), z x4), z x10)
\end{granule}
\item vec10:
\begin{granule}
vec10 : forall { a b : Type }
      . (a -> b) [10] 
      -> (((((((((a, a), a), a), a), a), a), a), a), a)
      -> (((((((((b, b), b), b), b), b), b), b), b), b)
vec10 [z] (((((((((x19, x20), x18), x16), x14), x12), x10), x8), p), v) = 
    (((((((((z x20, z v), z p), z x8), z x10), z x12), z x14), z x16), z x18), z x19)
\end{granule}
\item vec15:
\begin{granule}
vec15 : forall { a b : Type }
      . (a -> b) [15] 
      -> ((((((((((((((a, a), a), a), a), a), a), a), a), a), a), a), a), a), a)
      -> ((((((((((((((b, b), b), b), b), b), b), b), b), b), b), b), b), b), b)
vec15 [z] ((((((((((((((x29, x30), x28), x26), x24), x22), x20), x18), x16), x14), x12), x10), x8), p), v) = 
    ((((((((((((((z x30, z v), z p), z x8), z x10), z x12), z x14), z x16), z x18), z x20), z x22), z x24), z x26), z x28), z x29)
\end{granule}
\item vec20:
\begin{granule}
vec20 : forall { a b : Type }
      . (a -> b) [20] 
      -> (((((((((((((((((((a, a), a), a), a), a), a), a), a), a), a), a), a), a), a), a), a), a), a), a)
      -> (((((((((((((((((((b, b), b), b), b), b), b), b), b), b), b), b), b), b), b), b), b), b), b), b)
vec20 [z] (((((((((((((((((((x39, x40), x38), x36), x34), x32), x30), x28), x26), x24), x22), x20), x18), x16), x14), x12), x10), x8), p), v) = 
    (((((((((((((((((((z x40, z v), z p), z x8), z x10), z x12), z x14), z x16), z x18), z x20), z x22), z x24), z x26), z x28), z x30), z x32), z x34), z x36), z x38), z x39)
\end{granule}
\end{enumerate}

\subsection{Misc}
\begin{enumerate}
\item split$\oplus$:
\begin{granule}
data Either a b where Left a | Right b

splitPlus : forall { a b c : Type }
          . b [2..3] 
          -> Either a c 
          -> Either (a, b [2..2]) (c, b [3..3])
splitPlus [z] (Right x4) = Right (x4, [z]);
splitPlus [z] (Left x3) = Left (x3, [z])
\end{granule}
\item split$\otimes$:
\begin{granule}
splitPair : forall { a : Type }
          . (a -> a -> a) [0..2] 
          -> a [10..10] 
          -> (a [2..2], a [6..6])
splitPair [z] [u] = ([(z u) u], [u])
\end{granule}
\item share:
\begin{granule}
share : forall { a : Type }
      . (a -> a -> a) [0..2] 
      -> a [10..10] 
      -> (a [2..2], a [6..6])
share [z] [u] = ([(z u) u], [u])
\end{granule}
\item Exm.~\ref{exm:security}:
\begin{granule}
dontLeak : forall { a b : Type }
         . (a [Public], a [Private]) 
         -> ((a, ()) [Public] -> b)
         -> b
dontLeak ([w], [v]) y = y [(w, ())]
\end{granule}
\end{enumerate}

\section{Synthesised Programs for the Fully Graded Synthesis Calculus}
\label{sec:graded-benchmarks}
This section includes the synthesised programs, their synthesis contexts, and
examples used for the benchmarking problems in
Section~\ref{section:graded-base-evaluation}. The context of each synthesised
program is listed by the program's \granin{spec}. If the program has no
\granin{spec}, then synthesis is occurring in an empty context.

For each program we list the examples required to synthesise the correct result
in the Graded case, and the additional examples required to synthesise the same
program without grades (i.e. in the Cartesian setting). See 
Section~\ref{section:graded-base-evaluation} for further details.

\subsection{List}
\begin{enumerate}
\item append: 
\begin{granule}
language GradedBase

data List a = Nil | Cons a (List a)
    
append : forall { a : Type }
       . (List a) %1 
       -> a %1 
       -> List a
append x y = (Cons y) x
\end{granule}
with no Graded examples and Cartesian example(s):
\begin{granule}
append (Cons 1 Nil) 2 = (Cons 2 (Cons 1 Nil));
\end{granule}
\item concat:
\begin{granule}
language GradedBase 

data List a = Cons a (List a) | Nil
    
concat : forall { a : Type }
       . (List a) %1..Inf 
       -> (List a) %1..Inf 
       ->  List a
spec 
    concat %0..Inf
concat Nil y = y;
concat (Cons z u) y = (Cons z) ((concat u) y)
\end{granule}
with no Graded examples and Cartesian examples(s):
\begin{granule}
concat (Cons 0 Nil) Nil = (Cons 0 Nil);                                                                        
concat (Cons 0 Nil) (Cons 1 Nil) = (Cons 0 (Cons 1 Nil));                                                       
concat (Cons 0 (Cons 1 (Cons 2 Nil))) (Cons 3 (Cons 4 Nil)) = Cons 0 (Cons 1 (Cons 2 (Cons 3 (Cons 4 Nil))));
\end{granule}
\item empty: 
\begin{granule}
language GradedBase

data List a = Nil | Cons a (List a) 

empty : forall { a b : Type } . () -> List a
empty () = Nil
\end{granule}
\item snoc: 
\begin{granule}
language GradedBase

data List a = Nil | Cons a (List a)

data N = S N | Z

snoc : forall { a : Type }
     . (List a) %1..Inf 
     -> a %1..Inf 
     -> List a
spec 
    snoc %0..Inf
snoc x y = 
    (case x of
      Nil -> (Cons y) x;
      Cons z u -> (Cons z) ((snoc u) y))
\end{granule}
with Graded example(s):
\begin{granule}
snoc (Cons Z Nil) (S Z) = (Cons Z (Cons (S Z) Nil));
\end{granule}
\item drop: 
\begin{granule}
language GradedBase

data List a = Cons a (List a) | Nil
    
data N = S N | Z
        
drop : forall { a : Type } . N %0..Inf -> List (a) %0..Inf -> List a
spec 
    drop % 0..Inf
drop x y = 
    (case y of
        Nil -> 
    (case x of
        Z -> y;
        S z -> (drop z) y);
        Cons p q -> 
    (case x of
        Z -> q;
        S x8 -> q))
\end{granule}
with Graded example(s): 
\begin{granule}
drop (S Z) (Cons (S Z) (Cons Z Nil)) = Cons Z Nil; 
\end{granule}
\item flatten: 
\begin{granule}
language GradedBase 

data List a = Cons a (List a) | Nil
    
append : forall { a : Type } 
       . (List a) %1..Inf 
       -> (List a) %1..Inf 
       ->  List a
append Nil y = y;
append (Cons z u) y = (Cons z) ((append u) y)
    
flatten : forall { a : Type } . (List (List a)) %0..Inf -> (List a)
spec 
    flatten % 0..Inf , append %0..Inf
flatten Nil = (append Nil) Nil;
flatten (Cons u v) = (append u) (flatten v)
\end{granule}
with Graded example(s):
\begin{granule}
flatten (Cons (Cons 1 Nil) (Cons (Cons 1 Nil) Nil)) = Cons 1 (Cons 1 Nil);
\end{granule}
\item bind: 
\begin{granule}
language GradedBase

data List a = Nil | Cons a (List a) 

data N = S N | Z

data Bool = True | False; 

append : forall { a : Type } 
       . (List a) %1..Inf 
       -> (List a) %1..Inf 
       ->  List a
append Nil y = y;
append (Cons z u) y = (Cons z) ((append u) y)

concat : forall { a : Type } . (List (List a)) %1..Inf -> (List a)
concat Nil = Nil;
concat (Cons u v) = (append u) (concat v)

map : forall { a b : Type }
    . (a %1..Inf -> b) %0..Inf 
    -> List a %1..Inf 
    -> List b
map x Nil = Nil;
map x (Cons z u) = (Cons (x z)) ((map x) u)

isEven : N %1..Inf -> List N  
isEven Z = Nil;
isEven (S Z) = Cons (S Z) Nil;
isEven (S (S z)) = concat (Cons (isEven z) Nil)

bind : forall { a b : Type }
     . List a %1..Inf 
     -> (a %1..Inf -> List b) %0..Inf 
     -> List b
spec 
    map %1..Inf, concat %1..Inf
bind x y = concat ((map (\w -> w)) x)
\end{granule}
with no Graded examples and Cartesian example(s):
\begin{granule}
bind (Cons Z Nil) isEven = Nil;
bind (Cons (S Z) Nil) isEven = (Cons (S Z) Nil);
\end{granule}
\item return: 
\begin{granule}
language GradedBase

data List a =  Cons a (List a) | Nil 

return : forall { a b : Type } . a -> List a
return x = (Cons x) Nil
\end{granule}
with no Graded examples and Cartesian example(s):
\begin{granule}
return 1 = Cons 1 Nil;
\end{granule}
\item inc: 
\begin{granule}
language GradedBase

data List a = Cons a (List a) | Nil
    
data N = S N | Z
    
map : (List N) %1..Inf 
    -> (N %1..Inf -> N) %0..Inf 
    -> (List N)
map Nil f = Nil; 
map (Cons x xs) f = (Cons (f x) (map xs f))
    
inc : forall a . (List N) %1..Inf -> (List N)
spec
    map %1..Inf
inc x = (map x) (\u -> S u)
\end{granule}
with Graded example(s):
\begin{granule}
inc (Cons (S Z) Nil) = (Cons (S (S Z)) Nil);
\end{granule}
\item head:
\begin{granule}
language GradedBase

data List a = Cons a (List a) | Nil 
    
head : forall { a : Type } . (List a) %0..1 -> a %0..1 -> a
head Nil y = y;
head (Cons z u) y = z
\end{granule}
with Graded example(s):
\begin{granule}
head (Cons 1 (Cons 2 Nil)) 2 = 1;
\end{granule}
\item tail:
\begin{granule}
language GradedBase

data List a = Cons a (List a) | Nil 

tail : forall { a : Type } . List a %0..1 -> List a
tail Nil = Nil;
tail (Cons y z) = z
\end{granule}
with Graded example(s):
\begin{granule}
tail (Cons 1 (Cons 2 Nil)) = Cons 2 Nil;
\end{granule}
\item last: 
\begin{granule}
language GradedBase

data List a = Cons a (List a) | Nil
    
data Maybe a = Just a | Nothing    
    
last : forall { a : Type } . (List a) %0..Inf -> Maybe a 
spec
    last %0..Inf
last Nil = Nothing;
last (Cons y z) = 
    (case z of
        Nil -> last z;
        Cons v w -> Just v)
\end{granule}
with Graded example(s):
\begin{granule}
last (Cons 1 (Cons 2 Nil)) = Just 2;
\end{granule}
and Cartesian example(s):
\begin{granule}
last (Cons 1 Nil) = Just 1;
\end{granule}
\item length: 
\begin{granule}
language GradedBase 

data List a = Cons a (List a) | Nil 
    
data N = S N | Z
    
length : forall { a : Type } . List a %0..Inf -> N 
spec
    length %0..Inf
length Nil = Z;
length (Cons y z) = S (length z)
\end{granule}
with Graded example(s):
\begin{granule}
length (Cons 1 (Cons 1 Nil)) = S (S Z);
\end{granule}
\item map: 
\begin{granule}
language GradedBase

data List a = Nil | Cons a (List a) 
    
data Bool = True | False; 
    
neg : Bool %1..Inf -> Bool 
neg True = False;
neg False = True 
    
map : forall { a b : Type } 
    . (a % 1..Inf -> b) %0..Inf 
    -> List a %1..Inf 
    -> List b
spec 
    map % 0..Inf
map x Nil = Nil;
map x (Cons z u) = (Cons (x z)) ((map x) u)
\end{granule}
with no Graded examples and Cartesian example(s):
\begin{granule}
map neg (Cons True Nil) = Cons False Nil;
\end{granule}
\item replicate5: 
\begin{granule}
language GradedBase

data List a =  Cons a (List a) | Nil 

replicate5 : forall { a : Type } . a %5 -> List a 
replicate5 x = (Cons x) ((Cons x) ((Cons x) ((Cons x) ((Cons x) Nil))))
\end{granule}
with no Graded examples and Cartesian example(s):
\begin{granule}
replicate5 1 = Cons 1 (Cons 1 (Cons 1 (Cons 1 (Cons 1 Nil))));
\end{granule}
\item replicate10: 
\begin{granule}
language GradedBase

data List a =  Cons a (List a) | Nil 

replicate10 : forall { a : Type } . a %10 -> List a 
replicate10 x = (Cons x) ((Cons x) ((Cons x) ((Cons x) ((Cons x) ((Cons x) ((Cons x) ((Cons x) ((Cons x) ((Cons x) Nil)))))))))
\end{granule}
with no Graded examples and Cartesian example(s);
\begin{granule}
replicate10 1 = (Cons 1 (Cons 1 (Cons 1 (Cons 1 (Cons 1 (Cons 1 (Cons 1 (Cons 1 (Cons 1 (Cons 1 Nil))))))))));
\end{granule}
\item replicateN: 
\begin{granule}
language GradedBase

data List a =  Cons a (List a) | Nil 

data N = S N | Z
    
replicateN : forall { a : Type }
           . N %0..Inf 
           -> a %0..Inf 
           -> List a
spec
    replicateN % 0..Inf
replicateN Z y = Nil;
replicateN (S z) y = (Cons y) ((replicateN z) y)
\end{granule}
with Graded example(s):
\begin{granule}
replicateN (S (S Z)) 2 = (Cons 2 (Cons 2 Nil));
\end{granule}
\item stutter:
\begin{granule}
language GradedBase

data List a = Cons a (List a) | Nil

stutter : forall { a : Type } . List (a [2]) %1..Inf -> List a
spec
    stutter % 0..Inf
stutter Nil = Nil;
stutter (Cons [u] z) = (Cons u) ((Cons u) (stutter z))
\end{granule}
\item sum:
\begin{granule}
language GradedBase 

data N = S N | Z 

data List a = Cons a (List a) | Nil 

fold : List N %0..Inf 
     -> (N % 1..Inf 
     -> N % 1..Inf -> N) %0..Inf 
     -> N %0..Inf -> N 
fold Nil f acc = acc;
fold (Cons x xs) f acc =  fold xs f (f acc x)

add : N %1..Inf -> N %1..Inf -> N
add Z n2 = n2; 
add (S n1) n2 = S (add n1 n2)

sum : List N %0..Inf -> N 
spec 
    fold %0..Inf, add %0..Inf
sum x = ((fold x) (\p -> \q -> (add p) q)) ((add Z) Z)
\end{granule}
with Graded example(s):
\begin{granule}
sum (Cons (S Z) (Cons (S Z) Nil)) = (S (S Z));
\end{granule}
and Cartesian example(s):
\begin{granule}
sum (Cons (S Z) (Cons (S Z) (Cons (S Z) Nil))) = (S (S (S Z)));
\end{granule}
\end{enumerate}
\subsection{Stream}
\begin{enumerate}
\item build: 
\begin{granule}
language CBN 
language GradedBase

data Stream a = Next a (Stream a) 

ones : () %1..1 -> Stream Int
ones () = Next 1 (ones ())

head : forall { a : Type } . Stream a %0..1 -> a 
head (Next x xs) = x

build : forall { a : Type } . a %1..1 -> (Stream a) %1..1 -> Stream a
build x y = (Next x) y
\end{granule}
with no Graded examples and Cartesian example(s):
\begin{granule}
head (build 2 (ones ())) = 2;
\end{granule}
\item map: 
\begin{granule}
language CBN
language GradedBase 

data Stream a = Next a (Stream a) 

data Bool = True | False

trues : () %1..Inf -> Stream Bool
trues () = Next True (trues ())

neg : Bool %1..Inf -> Bool
neg True = False; 
neg False = True

head : forall { a : Type } . Stream a %0..Inf -> a 
head (Next x xs) = x

map : forall { a b : Type }
    . Stream a %1..Inf 
    -> (a %1..Inf -> b) %1..Inf 
    -> Stream b
spec 
    map % 1..Inf
map (Next z u) y = (Next (y z)) ((map_stream u) y)
\end{granule}
with no Graded examples and Cartesian example(s):
\begin{granule}
head (map_stream (trues ()) neg) = False;
\end{granule}
\item take1: 
\begin{granule}
language CBN 
language GradedBase 
    
data Stream a = Next a (Stream a) 

data Bool = True | False
    
ones : () %1..1 -> Stream Int
ones () = Next 1 (ones ())
    
head : forall { a : Type } . (Stream a) %0..1 -> a
head (Next x _) = x
    
take1 : forall { a : Type } . Stream a %0..1 -> a 
take1 (Next y z) = y
\end{granule}
with no Graded examples and Cartesian example(s):
\begin{granule}
take1 (Next 2 (ones ())) = 2;
\end{granule}
\item take2: 
\begin{granule}
language CBN 
language GradedBase 

data Stream a = Next a (Stream a) 
data Bool = True | False

ones : () %1..1 -> Stream Int
ones () = Next 1 (ones ())

head : forall { a : Type } . (Stream a) %0..1 -> a
head (Next x _) = x

take2 : forall { a : Type } . Stream a %0..1 -> (a, a)
take2 (Next y (Next u v)) = (u, y)
\end{granule}
with no Graded examples and Cartesian example(s):
\begin{granule}
take2 (Next 2 (ones ())) = (2, 1);
\end{granule}
\item take3: 
\begin{granule}
language CBN 
language GradedBase 

data Stream a = Next a (Stream a) 

data Bool = True | False

ones : () %1..1 -> Stream Int
ones () = Next 1 (ones ())

head : forall { a : Type } . (Stream a) %0..1 -> a
head (Next x _) = x

take3 : forall { a : Type } . Stream a %0..1 -> (a, (a, a))
take3 (Next y (Next u (Next w p))) = (y, (w, u))
\end{granule}
with no Graded examples and Cartesian example(s):
\begin{granule}
take3 (Next 3 (Next 2 (ones ()))) = (3, (2, 1));
\end{granule}
\end{enumerate}
\subsection{Bool}
\begin{enumerate}
\item neg: 
\begin{granule}
language GradedBase

data Bool = True | False

neg : Bool %1 -> Bool
neg True = False;
neg False = True
\end{granule}
with Graded example(s):
\begin{granule}
neg True = False;
neg False = True;
\end{granule}
\item and: 
\begin{granule}
language GradedBase

data Bool = True | False

and : Bool %1 -> Bool %1 -> Bool
and True True = True;
and False True = False;
and True False = False;
and False False = False
\end{granule}
with Graded example(s):
\begin{granule}
and True True = True;
and False True = False;
and True False = False;
and False False = False;
\end{granule}
\item impl: 
\begin{granule}
language GradedBase

data Bool = True | False

impl : Bool %1 -> Bool %1 -> Bool
impl True True = True;
impl True False = False;
impl False True = True;
impl False False = True
\end{granule}
with Graded example(s):
\begin{granule}
impl True True = True;
impl True False = False;
impl False True = True;
impl False False = True;
\end{granule}
\item or: 
\begin{granule}
language GradedBase

data Bool = True | False

or : Bool %1 -> Bool %1 -> Bool
or True True = True;
or False True = True;
or True False = True;
or False False = False
\end{granule}
with Graded example(s):
\begin{granule}
or True True = True;
or False True = True;
or True False = True;
or False False = False
\end{granule}
\item xor: 
\begin{granule}
language GradedBase

data Bool = True | False

xor : Bool %1 -> Bool %1 -> Bool
xor True True = False;
xor False True = True;
xor True False = True;
xor False False = False
\end{granule}
with Graded example(s):
\begin{granule}
xor True True = False;
xor False True = True;
xor True False = True;
xor False False = False
\end{granule}
\end{enumerate}
\subsection{Maybe}
\begin{enumerate}
\item bind: 
\begin{granule}
language GradedBase

data Maybe a = Just a | Nothing

data N = S N | Z

data Bool = True | False; 

isEven : N %1..Inf -> Maybe N  
isEven Z = Nothing;
isEven (S Z) = Just (S Z);
isEven (S (S z)) = 
    case isEven z of 
        Nothing -> Nothing;
        Just (S Z) -> Just (S Z)

bind : forall { a b : Type }
     . Maybe a %1..1 
     -> (a %1..1 -> Maybe b) %0..1 
     -> Maybe b
bind Nothing y = Nothing;
bind (Just z) y = y z
\end{granule}
with no Graded example(s) and Cartesian example(s):
\begin{granule}
bind (Just (S Z)) isEven = Just (S Z);
\end{granule}
\item fromMaybe: 
\begin{granule}
language GradedBase

data Maybe a = Nothing | Just a

fromMaybe : forall { a : Type } . Maybe a %(1..1) -> a %(0..1) -> a
fromMaybe Nothing y = y;
fromMaybe (Just z) y = z
\end{granule}
with no Graded example(s) and Cartesian example(s):
\begin{granule}
fromMaybe  Nothing 1 = 1;
fromMaybe (Just 1) 2 = 1;
\end{granule}
\item return: 
\begin{granule}
language GradedBase

data Maybe a = Nothing | Just a

return : forall { a : Type } . a -> Maybe a
return x = Just x
\end{granule}
\item isJust: 
\begin{granule}
language GradedBase

data Maybe a = Just a | Nothing 

data Bool = True | False 

isJust : forall { a : Type } . (Maybe a) %0..1 -> Bool
isJust Nothing = False;
isJust (Just y) = True
\end{granule}
with Graded example(s):
\begin{granule}
isJust (Just 1) = True;
isJust Nothing = False;
\end{granule}
\item isNothing: 
\begin{granule}
language GradedBase

data Maybe a = Just a | Nothing 
    
data Bool = True | False 
    
isNothing : forall { a : Type } . (Maybe a) %0..1 -> Bool
isNothing Nothing = True;
isNothing (Just y) = False
\end{granule}
with Graded example(s):
\begin{granule}
isNothing (Just 1) = False;
isNothing Nothing = True;
\end{granule}
\item map: 
\begin{granule}
language GradedBase

data Maybe a = Nothing | Just a

data N = S N | Z
data Bool = True | False

isOne : N %0..1 -> Bool 
isOne (S Z) = True;
isOne _ = False

map : forall { a b : Type }
    . (a -> b) %(0..1) 
    -> (Maybe a) %(1..1) 
    -> Maybe b
map x Nothing = Nothing;
map x (Just z) = Just (x z)
\end{granule}
with no Graded examples and Cartesian example(s):
\begin{granule}
map isOne (Just (S Z)) = Just True;
\end{granule}
\item mplus: 
\begin{granule}
language GradedBase

data Maybe a = Nothing | Just a

mplus : forall { a b : Type }
      . Maybe a %(0..1) 
      -> Maybe b %(0..1) 
      -> Maybe (a, b)
mplus Nothing Nothing = Nothing;
mplus (Just z) Nothing = Nothing;
mplus Nothing (Just v) = Nothing;
mplus (Just w) (Just v) = Just (w, v)
\end{granule}
with Graded example(s):
\begin{granule}
mplus (Just 1) (Just 2) = Just (1, 2);
\end{granule}
\end{enumerate}
\subsection{Nat}
\begin{enumerate}
\item isEven: 
\begin{granule}
language GradedBase 

data N = S N | Z

data Bool = True | False

isEven : N %1..Inf -> Bool  
spec 
    isEven % 0..Inf
isEven Z = True;
isEven (S Z) = False;
isEven (S (S z)) = isEven z
\end{granule}
with Graded example(s):
\begin{granule}
isEven (S (S Z)) = True;
isEven (S (S (S Z))) = False;
\end{granule}
\item pred: 
\begin{granule}
language GradedBase 

data N = S N | Z

pred : N %1 -> N 
pred Z = Z;
pred (S y) = y
\end{granule}
with Graded example(s):
\begin{granule}
pred (S (S Z)) = (S Z);
\end{granule}
\item succ: 
\begin{granule}
language GradedBase 

data N = S N | Z

succ : N %1 -> N 
succ x = S x
\end{granule}
with Graded example(s):
\begin{granule}
succ Z = (S Z);
\end{granule}
\item sum: 
\begin{granule}
language GradedBase 

data N = S N | Z

sum : N %1..Inf -> N %1..Inf -> N
spec 
    sum % 0..Inf
sum Z y = y;
sum (S z) y = S ((sum z) y)
\end{granule}
with Graded example(s):
\begin{granule}
sum (S Z) (S Z) = (S (S Z));
\end{granule}
and Cartesian example(s):
\begin{granule}
sum (S Z) Z = (S Z); 
sum (S (S (S (S Z)))) (S (S Z)) = (S (S (S (S (S (S Z))))));
\end{granule}
\end{enumerate}
\subsection{Tree}
\begin{enumerate}
\item map: 
\begin{granule}
language GradedBase

data Tree a = Leaf | Node (Tree a) a (Tree a)

data Bool = True | False

neg : Bool %1..Inf -> Bool
neg True = False; 
neg False = True

map : forall { a b : Type }
    . Tree a %1..Inf 
    -> (a %1..Inf -> b) %0..Inf 
    -> Tree b
spec
    map %0..Inf
map Leaf y = Leaf;
map (Node z u v) y = ((Node ((map z) y)) (y u)) ((map v) y)
\end{granule}
with no Graded examples and Cartesian example(s):
\begin{granule}
map (Node Leaf True Leaf) neg = (Node Leaf False Leaf);
\end{granule}
\item sutter: 
\begin{granule}
language GradedBase

data Tree a = Leaf | Node (Tree a) a (Tree a)

stutter : forall { a b : Type } . Tree (a [2]) %1..Inf -> Tree (a, a)
spec
    stutter %0..Inf
stutter Leaf = Leaf;
stutter (Node y [v] u) = ((Node (stutter y)) (v, v)) (stutter u)
\end{granule}
with no Graded examples and Cartesian example(s):
\begin{granule}
stutter (Node Leaf [1] Leaf) = (Node Leaf (1, 1) Leaf);
\end{granule}
\item sum: 
\begin{granule}
language GradedBase

data N = S N | Z
:W
data Tree a = Leaf | Node (Tree a) a (Tree a)

add : N %1..Inf -> N %1..Inf -> N
add Z y = y;
add (S z) y = S ((add z) y)

fold : Tree N %0..Inf 
     -> (N %1..Inf -> N %1..Inf -> N) %0..Inf
     -> N %0..Inf
     -> N 
fold Leaf f acc = acc;
fold (Node l x r) f acc = 
    fold l f (f x (fold r f acc))

sum : forall { a : Type } . Tree N %0..Inf -> N
spec 
    fold %1..Inf, add %1..Inf
sum x = (add Z) (((fold x) (\p -> \q -> (add p) q)) Z)
\end{granule}
with Graded example(s):
\begin{granule}
sum Leaf = Z;
sum (Node Leaf (S (S Z)) Leaf) = (S (S Z));
sum (Node (Node Leaf (S Z) (Node Leaf (S Z) Leaf)) (S (S Z)) Leaf) = (S (S (S (S Z))));
\end{granule}
\end{enumerate}
\subsection{Misc}
\begin{enumerate}
\item compose: 
\begin{granule}
language GradedBase

comp : forall {k : Coeffect, n m : k, a b c : Type} 
     . (a %m -> b) %n 
     -> (b %n -> c) %(1 : k) 
     -> a %(n * m) 
     -> c
comp x y z = y (x z)
\end{granule}
\item copy: 
\begin{granule}
language GradedBase

copy : forall { a : Type } . a %2 -> (a, a)
copy x = (x, x)
\end{granule}
\item push:
\begin{granule}
language GradedBase

push : forall { a b : Type, k : Coeffect, c : k } 
     . (a -> b) %c 
     -> a %c 
     -> b [c]
push x y = [x y]
\end{granule}
\end{enumerate}